pulse/lib/steel/pulse/Pulse.RuntimeUtils.fsti
@@ -62,3 +62,6 @@ val get_attributes (x:T.sigelt) : T.Tac (list R.term)
 val add_noextract_qual (x:T.sigelt) : (y:T.sigelt { x == y })
 
 val must_erase_for_extraction (g:env) (ty:T.term) : bool
+
+val magic : #a: Type -> unit -> GTot a
+val magic_s: #a: Type -> string -> GTot a
